Fixed definition of safe and sem_expr_shape, but broke proofs as a result :(

rupicola/io/STLC.fst
@@ -243,10 +243,6 @@ let get_ebool (b:bool) : closed_exp =
 (* Small-step operational semantics; strong / full-beta reduction is
    right to left  *)
 
-// define event that is correct wrt to histories
-// instead of refinement on event - use event_h (which is refinement with test_event h ev)
-// usually we do not look at the history
-// this needs to be with respect to the history (the local trace here is the singleton event)
 noeq
 type step : closed_exp -> closed_exp -> (h:history) -> option (event_h h) -> Type =
   | AppRight :
@@ -388,7 +384,6 @@ type steps : closed_exp -> closed_exp -> (h:history) -> local_trace h -> Type =
            steps e2 e3 (if Some? oev then (Some?.v oev)::h else h) lt ->
            steps e1 e3 h (if Some? oev then [Some?.v oev] @ lt else lt)
 
-// how would we check the compatability of two histories? saying that there exists an ordering of the events that is well-formed?
 let rec lem_steps_transitive_constructive
   (#e1 #e2 #e3:closed_exp) 
   (#h:history)
@@ -396,74 +391,25 @@ let rec lem_steps_transitive_constructive
   (st12:steps e1 e2 h lt1)
   (st23:steps e2 e3 (h++lt1) lt2)
   : Tot (steps e1 e3 h (lt1 @ lt2)) (decreases st12)
-  = admit ()   
-  (*match st12 with
-  | SRefl _ -> st23
-  | STrans #f1 #f1' #f2 #lt_f1'_f2 #oev f1_f1'_step f1'_f2_steps -> begin
-    let e1 = f1 in
-    let e2 = f2 in
-    let tr12 = (if Some? oev then (lt_f1'_f2 @ [Some?.v oev]) else lt_f1'_f2) in
-    match oev with
-    | Some ev -> begin
-      assert (tr12 == (lt_f1'_f2 @ [ev]));
-      assert (tr12 @ tr23 == (lt_f1'_f2 @ [ev]) @ tr23);
-      assume (tr12 @ tr23 == lt_f1'_f2 @ ([ev] @ tr23));
-      assume (well_formed_local_trace (List.rev lt_f1'_f2) tr23);
-      let steps23 : steps e2 e3 tr23 = st23 in
-      let result : steps f1' e3 (lt_f1'_f2 @ tr23) = lem_steps_transitive_constructive f1'_f2_steps st23 in
-      admit ()
-      end
-    | None -> begin
-      STrans f1_f1'_step (lem_steps_transitive_constructive f1'_f2_steps st23)
-      end
-    end*)
-
-  (*= match st12 with
-    | SRefl _ -> st23
-    | STrans #f1 #f1' #f2 #lt #oev f1_f1'_step f1'_f2_steps -> begin
-      let e1 = f1 in
-      let e2 = f2 in
-      let tr12 = (if Some? oev then (lt @ [Some?.v oev]) else lt) in
-      match oev with
-      | Some ev -> begin
-        assert (tr12 == (lt @ [ev]));
-        assume (well_formed_local_trace (List.rev lt) tr23);
-        
-        STrans #_ #_ #_ #((lt @ [ev]) @ tr23) f1_f1'_step (lem_steps_transitive_constructive f1'_f2_steps st23)
-        end
-      | None -> begin
-        assert (tr12 == lt);
-        STrans f1_f1'_step (lem_steps_transitive_constructive f1'_f2_steps st23)
-        end
-      end*)
-    
-    (*e1_can_step st12' -> begin
-      match get_oev e1_can_step with
-      | Some ev -> begin
-        let tr12' = get_lt st12' in
-        assume (well_formed_local_trace (List.rev tr12') tr23);
-        STrans e1_can_step (lem_steps_transitive_constructive st12' st23)
-        end
-      | None -> begin
-        STrans e1_can_step (lem_steps_transitive_constructive st12' st23)
-        end
-      end*)
+  = match st12 with
+    | SRefl _ h -> st23
+    | STrans e1_can_step st12' ->
+      STrans e1_can_step (lem_steps_transitive_constructive st12' st23)
 
 open FStar.Squash
+
+let get_event_trace (#h:history) (oev:option (event_h h)) : local_trace h = 
+  if Some? oev then [Some?.v oev] else []
 
 let lem_step_implies_steps (e e':closed_exp) (h:history) (oev:option (event_h h)) :
   Lemma
     (requires step e e' h oev)
-    (ensures steps e e' h (if Some? oev then [Some?.v oev] else [])) =
-    admit ()
-  (*introduce forall e e'. step e e' oev ==> steps e e' (if Some? oev then ([] @ [Some?.v oev]) else []) with
-    begin
-    introduce step e e' oev ==> steps e e' (if Some? oev then ([] @ [Some?.v oev]) else []) with h.
-      begin
-      bind_squash #(step e e' oev) () (fun st ->
-      return_squash (STrans st (SRefl e')))
-      end
-    end*)
+    (ensures steps e e' h (get_event_trace oev)) =
+  introduce forall e e'. step e e' h oev ==> steps e e' h (get_event_trace oev) with begin
+    introduce step e e' h oev ==> steps e e' h (get_event_trace oev) with _. begin
+      bind_squash #(step e e' h oev) () (fun st -> return_squash (STrans st (SRefl e' (h++(get_event_trace oev)))))
+    end
+  end
 
 let lem_steps_transitive 
   (e1 e2 e3:closed_exp)
@@ -478,32 +424,28 @@ let lem_steps_transitive
       return_squash (
         lem_steps_transitive_constructive st12 st23)))
 
-(*let lem_steps_irred_e_irred_e'_implies_e_e' (e:closed_exp{irred e}) (e':closed_exp{irred e'}) (lt:local_trace []) : Lemma
-  (requires steps e e' lt)
-  (ensures e == e') = admit ()*)
+let lem_steps_irred_e_irred_e'_implies_e_e' (#h:history) (e:closed_exp{irred e h}) (e':closed_exp{irred e' h}) (lt:local_trace h) : Lemma
+  (requires steps e e' h lt)
+  (ensures e == e') = admit ()
 
 let lem_steps_refl (e:closed_exp) (h:history) : Lemma (steps e e h []) [SMTPat (steps e e h [])] =
   FStar.Squash.return_squash (SRefl e h)
 
-let safe (e:closed_exp) : Type0 =
-  forall e' h lt. steps e e' h lt ==> is_value e' \/ can_step e' h
+let safe (e:closed_exp) (h:history) : Type0 =
+  forall (e':closed_exp) (lt:local_trace h). steps e e' h lt ==> is_value e' \/ can_step e' (h++lt)
 
 let lem_steps_preserve_safe (e e':closed_exp) (h:history) (lt:local_trace h) :
   Lemma
-    (requires (safe e) /\ (steps e e' h lt))
-    (ensures (safe e')) = admit ()
-  (*introduce forall e_f lt_e'_ef. steps e' e_f lt_e'_ef ==> is_value e_f \/ can_step e_f with
-    begin
-    introduce steps e' e_f lt_e'_ef ==> is_value e_f \/ can_step e_f with h.
-      begin
-      bind_squash #(steps e' e_f lt_e'_ef) () (fun st_f -> 
-      match st_f with
-      | SRefl e' -> ()
-      | STrans e'_can_step st_f' -> 
-        assume (well_formed_local_trace (List.rev lt_e_e') lt_e'_ef);
-        lem_steps_transitive e e' e_f lt_e_e' lt_e'_ef)
-      end
-    end*)
+    (requires (safe e h) /\ (steps e e' h lt))
+    (ensures (safe e' (h++lt))) = 
+  introduce forall e'' lt'. steps e' e'' (h++lt) lt' ==> is_value e'' \/ can_step e'' ((h++lt)++lt') with begin
+    introduce steps e' e'' (h++lt) lt' ==> is_value e'' \/ can_step e'' ((h++lt)++lt') with _. begin
+      bind_squash #(steps e' e'' (h++lt) lt') () (fun st -> 
+      match st with
+      | SRefl e' h -> ()
+      | STrans e'_can_step st_f' -> lem_steps_transitive e e' e'' h lt lt')
+    end
+  end
 
 (* We need syntactic types for this, or at least the top-level shape of types *)
 let sem_value_shape (t:typ) (e:closed_exp) : Tot Type0 =
@@ -513,31 +455,27 @@ let sem_value_shape (t:typ) (e:closed_exp) : Tot Type0 =
   | TArr t1 t2 -> ELam? e
   | TPair t1 t2 -> EPair? e
 
-let sem_expr_shape (t:typ) (e:closed_exp) : Tot Type0 =
-  forall e' h lt. steps e e' h lt ==> irred e' h ==> sem_value_shape t e'
+let sem_expr_shape (t:typ) (e:closed_exp) (h:history) : Tot Type0 =
+  forall (e':closed_exp) (lt:local_trace h). steps e e' h lt ==> irred e' (h++lt) ==> sem_value_shape t e'
 
 let lem_steps_preserve_sem_expr_shape (e e':closed_exp) (h:history) (lt:local_trace h) (t:typ) :
   Lemma
-    (requires (sem_expr_shape t e) /\ (steps e e' h lt))
-    (ensures (sem_expr_shape t e')) = admit ()
-  (*introduce forall e_f lt_e'_ef. steps e' e_f lt_e'_ef /\ irred e_f ==> sem_value_shape t e_f with
-    begin
-    introduce _  ==> sem_value_shape t e_f with h.
-      begin
-        bind_squash #(steps e' e_f lt_e'_ef) () (fun st_f ->
-        match st_f with
-        | SRefl e' -> ()
-        | STrans e'_can_step st_f' -> 
-          assume (well_formed_local_trace (List.rev lt_e_e') lt_e'_ef);
-          lem_steps_transitive e e' e_f lt_e_e' lt_e'_ef)
-      end
-    end*)
+    (requires (sem_expr_shape t e h) /\ (steps e e' h lt))
+    (ensures (sem_expr_shape t e' (h++lt))) =
+  introduce forall e'' lt'. steps e' e'' (h++lt) lt' /\ irred e'' ((h++lt)++lt') ==> sem_value_shape t e'' with begin
+    introduce _  ==> sem_value_shape t e'' with _. begin
+      bind_squash #(steps e' e'' (h++lt) lt') () (fun st ->
+      match st with
+      | SRefl e' h -> ()
+      | STrans e'_can_step st_f' -> lem_steps_transitive e e' e'' h lt lt')
+    end
+  end
 
 let can_step_eapp_when_safe (e1 e2:closed_exp) (t1 t2:typ) (h:history) : Lemma
   (requires
-    safe e1 /\
-    safe e2 /\
-    sem_expr_shape (TArr t1 t2) e1)
+    safe e1 h /\
+    safe e2 h /\
+    sem_expr_shape (TArr t1 t2) e1 h)
   (ensures (exists e' oev. step (EApp e1 e2) e' h oev))
   = 
   (**
@@ -589,9 +527,6 @@ let can_step_eapp_when_safe (e1 e2:closed_exp) (t1 t2:typ) (h:history) : Lemma
        Subsubcase irred e2. (From safe e2 we get is_value e2; but not needed by step.)
          So e = EApp (ELam e11) e2 -> subst_beta e2 e11 = e''. Return e11 e2. *)
 
-let get_event_trace (#h:history) (oev:option (event_h h)) : local_trace h = 
-  if Some? oev then [Some?.v oev] else []
-
 let rec destruct_steps_eapp
   (e1:closed_exp)
   (e2:closed_exp)
@@ -603,9 +538,9 @@ let rec destruct_steps_eapp
   (t2:typ) :
   Pure (exp * value * (lt2:local_trace h & (lt1:local_trace (h++lt2) & local_trace (((h++lt2)++lt1)))))
     (requires irred e' (h++lt) /\ (** CH: needed, otherwise I can take zero steps; could be replaced by value e' *)
-      safe e1 /\
-      sem_expr_shape (TArr t1 t2) e1 /\
-      safe e2)
+      safe e1 h /\
+      sem_expr_shape (TArr t1 t2) e1 h /\
+      safe e2 h)
     (ensures fun (e11, e2', (| lt2, (| lt1, lt3 |) |)) ->
       steps e2 e2' h lt2 /\
       is_closed (ELam e11) /\
@@ -632,8 +567,15 @@ let rec destruct_steps_eapp
         lem_step_implies_steps (EApp e1 e2) (EApp e1' e2) h oev1;
         let lt1 : local_trace h = get_event_trace oev1 in
         lem_steps_preserve_safe e1 e1' h lt1;
+        assert (safe e2 (h++lt1));
+        lem_steps_preserve_safe e2 e2 h lt1;
+        assert (safe e1' (h++lt1));
         lem_steps_preserve_sem_expr_shape e1 e1' h lt1 (TArr t1 t2);
+        assert (sem_expr_shape (TArr t1 t2) e1' (h++lt1));
         let s2 : steps (EApp e1' e2) e' (h++lt1) lt23 = step_eapp_steps in
+        assert (irred e' ((h++lt1)++lt23));
+        assert (safe e1' (h++lt1));
+        //assume (safe e2 (h++lt1));
         let (e11, e2', (| _, (| lt1', lt3 |) |)) = destruct_steps_eapp e1' e2 e' (h++lt1) lt23 s2 t1 t2 in
         lem_steps_transitive e1 e1' (ELam e11) h lt1 lt1';
         lem_steps_transitive (EApp e1 e2) (EApp e1' e2) (subst_beta e2' e11) h lt1 lt1';
